aux/coredefs.v
@@ -1,0 +1,93 @@
+Require Import List.
+Import ListNotations.
+Require Import PeanoNat.
+Require Import Coq.omega.Omega.
+Require Import Coq.Numbers.NatInt.NZOrder.
+
+From VLG Require Import matcher.
+From VLG Require Import ltac.
+
+Definition Sigma := matcher.Sigma.
+Definition Sigma_dec := matcher.Sigma_dec.
+Definition String := matcher.String.
+
+Lemma String_dec : forall s s' : String, {s = s'} + {s <> s'}.
+Proof. decide equality. apply Sigma_dec. Qed.
+
+Definition State : Type := regex.
+Definition transition : Sigma -> State -> State := derivative.
+Definition accepts : String -> State -> bool := exp_matchb.
+Definition accepting : State -> bool:= nullable.
+
+Lemma accepts_nil: forall(fsm : State),
+    accepting fsm = accepts [] fsm.
+Proof.
+  intros fsm. reflexivity.
+Qed.
+
+Lemma accepts_transition : forall cand a fsm,
+    accepts cand (transition a fsm)
+    = accepts (a :: cand) fsm.
+Proof.
+  auto.
+Qed.
+
+Inductive eq_models : State -> regex -> Prop :=
+| SReq (fsm : State) (r : regex)
+       (H1 : forall(s : String), true = accepts s fsm <-> exp_match s r) :
+    eq_models fsm r.
+
+Definition init_state (r : regex) : State := r.
+Definition init_state_inv (fsm : State) : regex := fsm.
+(** Facts about inverting init_state **)
+Lemma invert_init_correct' : forall(r : regex) (s : String),
+    exp_match s (init_state_inv (init_state r)) <-> exp_match s r.
+Proof.
+  intros. split; auto.
+Qed.
+
+Definition Label : Type := String.
+Definition Prefix : Type := String.
+Definition Suffix : Type := String.
+Definition Token : Type := Label * Prefix.
+Definition Rule : Type := Label * regex.
+
+Lemma ru_dec : forall (ru1 ru2 : Rule), {ru1 = ru2} + {ru1 <> ru2}.
+Proof.
+  intros. destruct ru1. destruct ru2.
+  destruct (String_dec l l0); destruct (regex_dec r r0); subst; auto;
+    right; intros C; destruct n; inv C; auto.
+Qed.
+
+Definition sRule : Type := Label * State.
+
+(** Facts about accepts/accepting **)
+Lemma accepts_matches : forall(s : String) (fsm : State),
+    true = accepts s fsm <-> exp_match s (init_state_inv fsm).
+Proof.
+  intros. split; intros; apply match_iff_matchb; auto.
+Qed.
+
+(* no external depends after this *)
+Lemma accepting_nilmatch : forall fsm,
+    true = accepting fsm
+    <-> exp_match [] (init_state_inv fsm).
+Proof.
+  intros. split; intros.
+  - apply accepts_matches. rewrite <- accepts_nil. auto.
+  - apply accepts_matches in H. rewrite accepts_nil. auto.
+Qed.
+
+Lemma inv_eq_model : forall(fsm : State),
+    eq_models fsm (init_state_inv fsm).
+Proof.
+  intros fsm. apply SReq. intros s. rewrite accepts_matches. split; auto.
+Qed.
+
+Lemma inv_transition : forall cand a fsm,
+    exp_match cand (init_state_inv (transition a fsm))
+    <-> exp_match (a :: cand) (init_state_inv fsm).
+Proof.
+  intros. repeat rewrite <- accepts_matches. rewrite accepts_transition.
+  split; auto.
+Qed.
