legacy/instance.v
@@ -1,0 +1,1 @@
+From VLG Require Import lexer.
