prefixer.v
@@ -1,0 +1,84 @@
+Require Import List.
+Import ListNotations.
+Require Import PeanoNat.
+Require Import Coq.omega.Omega.
+
+From VLG Require Import ltac.
+From VLG Require Import coredefs.
+From VLG Require Import spec.
+From VLG Require Import matcher.
+
+Fixpoint max_pref_fn (s : String) (state : State) : option (Prefix * Suffix):=
+  match s with
+  (* in a regex approach, accepting := nullable *)
+  | [] => if accepting state then Some ([],[]) else None
+  | a :: s' =>
+    let
+      (* in a regex approach, transition := derivative *)
+      state' := transition a state in
+    let
+      mpxs := max_pref_fn s' state' in
+
+    match mpxs with
+    | None => if (accepting state') then Some ([a], s') else
+               if (accepting state) then Some ([], s) else
+                 None
+    | Some (p, q) => Some (a :: p, q)
+    end
+  end.
+
+Definition extract_fsm_for_max (code : String) (sru : (Label * State)) :=
+  match sru with
+    (a, fsm) => (a, max_pref_fn code fsm)
+  end.
+
+Definition max_prefs (code : String) (erules : list (Label * State)) :=
+  map (extract_fsm_for_max code) erules.
+
+(* prefixes closest to the head are preferred *)
+Definition longer_pref (apref1 apref2 : Label * (option (Prefix * Suffix)))
+  : Label * (option (Prefix * Suffix)) :=
+  match apref1, apref2 with
+  | (_, None), (_, _) => apref2
+  | (_, _), (_, None) => apref1
+  (* This is finding the min right now... *)
+  | (_, Some (x, _)), (_, Some (y, _)) => if (length x) =? (length y)
+                                          then apref1 else
+                                            if (length x) <? (length y)
+                                            then apref2 else apref1
+  end.
+
+Lemma max_pref_fn_splits : forall code prefix suffix (fsm : State),
+    Some (prefix, suffix) = max_pref_fn code fsm -> code = prefix ++ suffix.
+Proof.
+  induction code as [| a s']; intros prefix suffix fsm H; simpl in H;
+    repeat dm; repeat inj_all; auto; try(discriminate).
+  symmetry in E. apply IHs' in E. rewrite E. auto.
+Qed.
+
+Lemma proper_suffix_shorter : forall code prefix suffix (fsm : State),
+    prefix <> []
+    -> Some (prefix, suffix) = max_pref_fn code fsm
+    -> length suffix < length code.
+Proof.
+  intros code prefix suffix fsm. intros Hneq Heq.
+  apply max_pref_fn_splits in Heq. rewrite Heq.
+  replace (length (prefix ++ suffix)) with ((length prefix) + (length suffix)).
+  - apply Nat.lt_add_pos_l. destruct prefix.
+    + contradiction.
+    + simpl. omega.
+  - symmetry. apply app_length.
+Qed.
+
+Fixpoint max_of_prefs (mprefs : list (Label * (option (Prefix * Suffix))))
+  : Label * option (Prefix * Suffix) :=
+  match mprefs with
+  | [] => ([], @None (String * String))
+  | p :: ps => longer_pref p (max_of_prefs ps)
+  end.
+
+Lemma max_first_or_rest : forall ys x y,
+    x = max_of_prefs (y :: ys) -> x = y \/ x = max_of_prefs ys.
+Proof.
+  intros. simpl in H. unfold longer_pref in H. repeat dm.
+Qed.
