spec.v
@@ -1,0 +1,106 @@
+Require Import List.
+Import ListNotations.
+
+From VLG Require Import matcher.
+From VLG Require Import coredefs.
+
+Inductive is_prefix : String -> String -> Prop :=
+| pref_def p s
+           (H1 : exists q, p ++ q = s) :
+    is_prefix p s.
+
+Notation "p ++_= s" := (is_prefix p s) (at level 80).
+
+Inductive re_no_max_pref : String -> regex -> Prop :=
+| re_MP0 (s : String) (r : regex)
+         (H1 : forall cand, cand ++_= s -> ~(exp_match cand r)) :
+    re_no_max_pref s r.
+
+Inductive re_max_pref : String -> regex -> String -> Prop :=
+| re_MP1 (s p : String) (r : regex)
+         (H1 : p ++_= s)
+         (H2 : exp_match p r)
+         (H3 : forall(cand : String),
+             cand ++_= s
+             -> ((length cand) <= (length p)) \/ ~(exp_match cand r)) :
+    re_max_pref s r p.
+
+Inductive no_max_pref : String -> State -> Prop :=
+| MP0 (s : String) (fsm : State)
+      (H1 : exists(r : regex), eq_models fsm r /\ re_no_max_pref s r) :
+    no_max_pref s fsm.
+
+Inductive max_pref : String -> State -> String -> Prop :=
+| MP1 (s p : String) (fsm : State)
+      (H1 : exists(r : regex), eq_models fsm r /\ re_max_pref s r p) :
+    max_pref s fsm p.
+
+(* a rule is at index 0 if it's the first element of the list.
+   Otherwise a rule is at index n + 1 if it's at index n of the tail of the list *)
+Inductive at_index : Rule -> nat -> list Rule -> Prop :=
+| AI0 (ru h: Rule) (tl : list Rule)
+      (Heq : ru = h) :
+    at_index ru 0 (h :: tl)
+| AI1 (ru h: Rule) (n : nat) (tl : list Rule)
+      (IH : at_index ru n tl) :
+    at_index ru (S n) (h :: tl).
+
+(* n is the first index of a rule if no smaller index maps to that rule *)
+Inductive least_index : Rule -> nat -> list Rule -> Prop :=
+| LI1 (ru : Rule) (n : nat) (rus : list Rule)
+      (Hat : at_index ru n rus)
+      (Hnot : forall(n' : nat), n' < n -> ~(at_index ru n' rus)) :
+    least_index ru n rus.
+
+(* A rule is "earlier" than another if its first occurrence comes before
+   the first occurence of the other rule *)
+Inductive earlier_rule : Rule -> Rule -> list Rule -> Prop :=
+| ERu1 (ru1 ru2 : Rule) (rus : list Rule)
+       (H : forall(n1 n2 : nat),
+           least_index ru1 n1 rus
+           -> least_index ru2 n2 rus
+           -> n1 < n2) :
+    earlier_rule ru1 ru2 rus.
+
+Inductive first_token : String -> (list Rule) -> Token -> Prop :=
+(* l is Token.label, p is Token.value *)
+| FT1 (code : String) (p : Prefix) (l : Label) (r : regex) (rus : list Rule)
+      (Hnempt : p <> [])
+      (Hex : In (l, r) rus)
+      (Hmpref : re_max_pref code r p)
+      (* We can't produce longer prefixes from other rules *)
+      (Hout : forall(l' : String) (r' : regex) (p' : String),
+          length p' > length p
+          -> re_max_pref code r' p'
+          -> ~(In (l',r') rus)
+      )
+      (* If we can produce the prefix in some other way,
+           the rule used to do so most come later in the list *)
+      (Hlater : forall(r' : regex) (l' : String),
+          earlier_rule (l',r') (l, r) rus
+          -> In (l', r') rus
+          -> ~(re_max_pref code r' p)
+      ) :
+    first_token code rus (l, p).
+
+(* This definition accounts for inputs that could not be entirely tokenized.
+   The list of tokens must match some prefix and the unprocessed suffix
+   must match s1 *)
+Inductive tokenized (rus : list Rule) : String -> list Token -> String -> Prop :=
+| Tkd0 (code : String)
+       (H : forall(t : Token), first_token code rus t -> snd t = []) :
+    (* If no tokens can be produced from the input,
+       then the input is tokenized by the empty list
+       of tokens and itself *)
+    tokenized rus code [] code
+| Tkd1 (p : Prefix) (s0 s1 : Suffix) (ts : list Token) (l : Label)
+       (* the first token matches the input *)
+       (H0 : first_token (p ++ s0 ++ s1) rus (l,p))
+       (* The rest of the tokens match the rest of the input *)
+       (IH : tokenized rus (s0 ++ s1) ts s1) :
+    tokenized rus (p ++ s0 ++ s1) ((l, p) :: ts) s1.
+
+Definition rules_is_function (rus : list Rule) :=
+  forall l r r', In (l, r) rus
+                 -> In (l, r') rus
+                 -> r = r'.
